Prove promise_step

src/localdrfra/RASimThread.v
@@ -74,13 +74,91 @@ Module RASimThread.
     .
 
 
-    (* sim_thread *)
+    Lemma future_stable_view
+          mem1 mem2 view
+          (CLOSED: Memory.closed_view view mem1)
+          (STABLE: stable_view mem1 view)
+          (MEM_FUTURE: Memory.future mem1 mem2):
+      stable_view mem2 view.
+    Proof.
+      ii. inv CLOSED. specialize (RLX loc). des.
+      exploit STABLE; eauto. i.
+      exploit Memory.future_get1; try exact RLX; eauto. i. des.
+      rewrite GET0 in *. inv GET. inv MSG_LE.
+      etrans; eauto.
+    Qed.
+
+    Lemma future_stable_tview
+          mem1 mem2 tview
+          (CLOSED: TView.closed tview mem1)
+          (STABLE: stable_tview mem1 tview)
+          (MEM_FUTURE: Memory.future mem1 mem2):
+      stable_tview mem2 tview.
+    Proof.
+      destruct tview. inv CLOSED. inv STABLE. ss.
+      econs; ss; eauto using future_stable_view.
+    Qed.
+
+    Lemma future_stable
+          e sc' mem'
+          (WF: Local.wf e.(Thread.local) e.(Thread.memory))
+          (STABLE: stable_thread e)
+          (SC: TimeMap.le e.(Thread.sc) sc')
+          (MEM_FUTURE: Memory.future e.(Thread.memory) mem')
+          (MEM_STABLE: stable_memory mem'):
+      stable_thread (Thread.mk lang e.(Thread.state) e.(Thread.local) sc' mem').
+    Proof.
+      destruct e, local. inv STABLE. inv WF. ss.
+      econs; i; ss; eauto using future_stable_tview.
+    Qed.
+
+
+    (* sim *)
 
     Definition reserve_only (promises: Memory.t): Prop :=
       forall loc from to val released
         (LOC: L loc)
         (PROMISE: Memory.get loc to promises = Some (from, Message.concrete val released)),
         False.
+
+    Inductive sim_tview (tview_src tview_tgt: TView.t): Prop :=
+    | sim_tview_intro
+        (REL: forall loc (LOC: ~ L loc),
+            tview_src.(TView.rel) loc = tview_tgt.(TView.rel) loc)
+        (CUR: tview_src.(TView.cur) = tview_tgt.(TView.cur))
+        (ACQ: tview_src.(TView.acq) = tview_tgt.(TView.acq))
+    .
+
+    Definition rel_write (e: ThreadEvent.t): option (Loc.t * Time.t) :=
+      match e with
+      | ThreadEvent.write loc from to val released ord =>
+        if Ordering.le Ordering.acqrel ord then Some (loc, to) else None
+      | ThreadEvent.update loc tsr to valr valw releasedr releasedw ordr ordw =>
+        if Ordering.le Ordering.acqrel ordw then Some (loc, to) else None
+      | _ => None
+      end.
+
+    (* Inductive rel_write (tr: Trace.t lang) (loc: Loc.t) (to: Time.t): Prop := *)
+    (* | rel_write_write *)
+    (*     e from val released ord *)
+    (*     (IN: List.In (e, ThreadEvent.write loc from to val released ord) tr) *)
+    (*     (ORD: Ordering.le Ordering.acqrel ord) *)
+    (* | rel_write_update *)
+    (*     e tsr valr valw releasedr releasedw ordr ordw *)
+    (*     (IN: List.In (e, ThreadEvent.update loc tsr to valr valw releasedr releasedw ordr ordw) tr) *)
+    (*     (ORD: Ordering.le Ordering.acqrel ordw) *)
+    (* . *)
+
+    Inductive sim_local (tr: Trace.t lang) (lc_src lc_tgt: Local.t): Prop :=
+    | sim_local_intro
+        (TVIEW: sim_tview lc_src.(Local.tview) lc_tgt.(Local.tview))
+        (PROMISES: lc_src.(Local.promises) = lc_tgt.(Local.promises))
+        (RESERVE: reserve_only lc_src.(Local.promises))
+        (REL_WRITES_NONE: forall loc to th e
+                            (IN: List.In (th, e) tr)
+                            (REL: rel_write e = Some (loc, to)),
+            Memory.get loc to lc_src.(Local.promises) = None)
+    .
 
     Inductive sim_message (loc: Loc.t): forall (msg_src msg_tgt: Message.t), Prop :=
     | sim_message_concrete
@@ -91,16 +169,16 @@ Module RASimThread.
         sim_message loc Message.reserve Message.reserve
     .
 
-    Inductive rel_write (tr: Trace.t lang) (loc: Loc.t) (to: Time.t): Prop :=
-    | rel_write_write
-        e from val released ord
-        (IN: List.In (e, ThreadEvent.write loc from to val released ord) tr)
-        (ORD: Ordering.le Ordering.acqrel ord)
-    | rel_write_update
-        e tsr valr valw releasedr releasedw ordr ordw
-        (IN: List.In (e, ThreadEvent.update loc tsr to valr valw releasedr releasedw ordr ordw) tr)
-        (ORD: Ordering.le Ordering.acqrel ordw)
-    .
+    Program Instance sim_message_Equivalence: forall loc, Equivalence (sim_message loc).
+    Next Obligation.
+      ii. destruct x; econs; eauto. des_ifs.
+    Qed.
+    Next Obligation.
+      ii. inv H; econs; eauto. des_ifs.
+    Qed.
+    Next Obligation.
+      ii. inv H; inv H0; ss; econs; eauto. des_ifs.
+    Qed.
 
     Inductive sim_memory (tr: Trace.t lang) (mem_src mem_tgt: Memory.t): Prop :=
     | sim_memory_intro
@@ -114,7 +192,9 @@ Module RASimThread.
             exists msg_src,
               <<GET_SRC: Memory.get loc to mem_src = Some (from, msg_src)>> /\
               <<MSG: sim_message loc msg_src msg_tgt>>)
-        (REL_WRITES: forall loc to (REL_WRITE: rel_write tr loc to),
+        (REL_WRITES: forall loc to th e
+                       (IN: List.In (th, e) tr)
+                       (REL: rel_write e = Some (loc, to)),
             exists from msg,
               <<GET_SRC: Memory.get loc to mem_src = Some (from, msg)>> /\
               <<GET_TGT: Memory.get loc to mem_tgt = Some (from, msg)>>)
@@ -126,11 +206,368 @@ Module RASimThread.
         (NORMAL_SRC: normal_thread e_src)
         (NORMAL_TGT: normal_thread e_tgt)
         (STATE: e_src.(Thread.state) = e_tgt.(Thread.state))
-        (TVIEW: e_src.(Thread.local).(Local.tview) = e_tgt.(Thread.local).(Local.tview))
-        (PROMISES_SRC: reserve_only e_src.(Thread.local).(Local.promises))
-        (PROMISES_TGT: reserve_only e_tgt.(Thread.local).(Local.promises))
+        (LOCAL: sim_local tr e_src.(Thread.local) e_tgt.(Thread.local))
         (SC: e_src.(Thread.sc) = e_tgt.(Thread.sc))
         (MEMORY: sim_memory tr e_src.(Thread.memory) e_tgt.(Thread.memory))
     .
+
+    Lemma sim_memory_closed_timemap
+          tr mem_src mem_tgt tm
+          (SIM: sim_memory tr mem_src mem_tgt)
+          (CLOSED_TGT: Memory.closed_timemap tm mem_tgt):
+      Memory.closed_timemap tm mem_src.
+    Proof.
+      inv SIM. ii.
+      specialize (CLOSED_TGT loc). des.
+      exploit COMPLETE; eauto. i. des. inv MSG.
+      eauto.
+    Qed.
+
+    Lemma sim_memory_closed_view
+          tr mem_src mem_tgt view
+          (SIM: sim_memory tr mem_src mem_tgt)
+          (CLOSED_TGT: Memory.closed_view view mem_tgt):
+      Memory.closed_view view mem_src.
+    Proof.
+      inv CLOSED_TGT. econs; eauto using sim_memory_closed_timemap.
+    Qed.
+
+    Lemma sim_memory_closed_opt_view
+          tr mem_src mem_tgt view
+          (SIM: sim_memory tr mem_src mem_tgt)
+          (CLOSED_TGT: Memory.closed_opt_view view mem_tgt):
+      Memory.closed_opt_view view mem_src.
+    Proof.
+      inv CLOSED_TGT; eauto using sim_memory_closed_view.
+    Qed.
+
+    Lemma sim_memory_closed_message
+          tr mem_src mem_tgt msg
+          (SIM: sim_memory tr mem_src mem_tgt)
+          (CLOSED_TGT: Memory.closed_message msg mem_tgt):
+      Memory.closed_message msg mem_src.
+    Proof.
+      inv CLOSED_TGT; eauto using sim_memory_closed_opt_view.
+    Qed.
+
+
+    (* step *)
+
+    (* Lemma promise *)
+    (*       tr promises1 mem1_src mem1_tgt *)
+    (*       loc from to msg promises2 mem2_tgt kind *)
+    (*       (SIM1: sim_memory tr mem1_src mem1_tgt) *)
+    (*       (REL_WRITES_NONE: forall loc to th e *)
+    (*                           (IN: List.In (th, e) tr) *)
+    (*                           (REL: rel_write e = Some (loc, to)), *)
+    (*           Memory.get loc to promises1 = None) *)
+    (*       (LE1_SRC: Memory.le promises1 mem1_src) *)
+    (*       (LE1_TGT: Memory.le promises1 mem1_tgt) *)
+    (*       (PROMISE_TGT: Memory.promise promises1 mem1_tgt loc from to msg promises2 mem2_tgt kind): *)
+    (*   exists mem2_src, *)
+    (*     <<PROMISE_SRC: Memory.promise promises1 mem1_src loc from to msg promises2 mem2_src kind>> /\ *)
+    (*     <<SIM2: sim_memory tr mem2_src mem2_tgt>>. *)
+    (* Proof. *)
+    (* Admitted. *)
+
+    Lemma sim_memory_add
+          tr mem1_src
+          mem1_tgt loc from to msg mem2_tgt
+          (SIM1: sim_memory tr mem1_src mem1_tgt)
+          (ADD_TGT: Memory.add mem1_tgt loc from to msg mem2_tgt):
+      exists mem2_src,
+        <<ADD_SRC: Memory.add mem1_src loc from to msg mem2_src>> /\
+        <<SIM2: sim_memory tr mem2_src mem2_tgt>>.
+    Proof.
+      inv SIM1.
+      exploit (@Memory.add_exists mem1_src loc from to msg).
+      { ii. inv LHS. inv RHS. ss.
+        exploit SOUND; eauto. i. des.
+        exploit Memory.add_get0; eauto. i. des.
+        exploit Memory.add_get1; eauto. i.
+        exploit Memory.get_ts; try exact GET0. i. des.
+        { subst. timetac. }
+        exploit Memory.get_ts; try exact x1. i. des.
+        { subst. timetac. }
+        exploit Memory.get_disjoint; [exact GET0|exact x1|..]. i. des.
+        { subst. congr. }
+        apply (x4 x); econs; eauto. }
+      { inv ADD_TGT. inv ADD. ss. }
+      { inv ADD_TGT. inv ADD. ss. }
+      i. des.
+      esplits; eauto. econs; i.
+      - revert GET_SRC. erewrite Memory.add_o; eauto. condtac; ss.
+        + i. des. inv GET_SRC.
+          erewrite Memory.add_o; eauto. condtac; ss.
+          esplits; eauto. refl.
+        + i. erewrite Memory.add_o; eauto. condtac; ss. eauto.
+      - revert GET_TGT. erewrite Memory.add_o; eauto. condtac; ss.
+        + i. des. inv GET_TGT.
+          erewrite Memory.add_o; eauto. condtac; ss.
+          esplits; eauto. refl.
+        + i. erewrite Memory.add_o; eauto. condtac; ss. eauto.
+      - exploit REL_WRITES; eauto. i. des.
+        erewrite Memory.add_o; eauto.
+        erewrite (@Memory.add_o mem2_tgt); eauto.
+        condtac; ss; eauto.
+        des. subst. esplits; eauto.
+    Qed.
+
+    Lemma sim_memory_split
+          tr mem1_src
+          mem1_tgt loc ts1 ts2 ts3 msg2 msg3 mem2_tgt
+          (SIM1: sim_memory tr mem1_src mem1_tgt)
+          (LOC: L loc = false)
+          (SPLIT_TGT: Memory.split mem1_tgt loc ts1 ts2 ts3 msg2 msg3 mem2_tgt):
+      exists mem2_src,
+        <<SPLIT_SRC: Memory.split mem1_src loc ts1 ts2 ts3 msg2 msg3 mem2_src>> /\
+        <<SIM2: sim_memory tr mem2_src mem2_tgt>>.
+    Proof.
+      inv SIM1.
+      exploit (@Memory.split_exists mem1_src loc ts1 ts2 ts3 msg2 msg3).
+      { exploit Memory.split_get0; eauto. i. des.
+        exploit COMPLETE; try exact GET0. i. des.
+        inv MSG; ss. rewrite LOC in *. subst. ss. }
+      { inv SPLIT_TGT. inv SPLIT. ss. }
+      { inv SPLIT_TGT. inv SPLIT. ss. }
+      { inv SPLIT_TGT. inv SPLIT. ss. }
+      i. des.
+      esplits; eauto. econs; i.
+      - revert GET_SRC. erewrite Memory.split_o; eauto. repeat condtac; ss; i.
+        + des. inv GET_SRC.
+          erewrite Memory.split_o; eauto. repeat condtac; ss.
+          esplits; eauto. refl.
+        + guardH o. des. inv GET_SRC.
+          erewrite Memory.split_o; eauto. repeat condtac; ss.
+          esplits; eauto. refl.
+        + erewrite Memory.split_o; eauto. repeat condtac; ss. eauto.
+      - revert GET_TGT. erewrite Memory.split_o; eauto. repeat condtac; ss; i.
+        + des. inv GET_TGT.
+          erewrite Memory.split_o; eauto. repeat condtac; ss.
+          esplits; eauto. refl.
+        + guardH o. des. inv GET_TGT.
+          erewrite Memory.split_o; eauto. repeat condtac; ss.
+          esplits; eauto. refl.
+        + erewrite Memory.split_o; eauto. repeat condtac; ss. eauto.
+      - exploit REL_WRITES; eauto. i. des.
+        erewrite Memory.split_o; eauto.
+        erewrite (@Memory.split_o mem2_tgt); eauto.
+        repeat condtac; ss; eauto.
+        + des. subst. esplits; eauto.
+        + guardH o. des. subst. esplits; eauto.
+    Qed.
+
+    Lemma sim_memory_lower
+          tr mem1_src
+          mem1_tgt loc from to msg1 msg2 mem2_tgt
+          (SIM1: sim_memory tr mem1_src mem1_tgt)
+          (LOC: L loc = false)
+          (LOWER_TGT: Memory.lower mem1_tgt loc from to msg1 msg2 mem2_tgt):
+      exists mem2_src,
+        <<LOWER_SRC: Memory.lower mem1_src loc from to msg1 msg2 mem2_src>> /\
+        <<SIM2: sim_memory tr mem2_src mem2_tgt>>.
+    Proof.
+      inv SIM1.
+      exploit (@Memory.lower_exists mem1_src loc from to msg1 msg2).
+      { exploit Memory.lower_get0; eauto. i. des.
+        exploit COMPLETE; eauto. i. des. inv MSG; ss.
+        rewrite LOC in *. subst. ss. }
+      { inv LOWER_TGT. inv LOWER. ss. }
+      { inv LOWER_TGT. inv LOWER. ss. }
+      { inv LOWER_TGT. inv LOWER. ss. }
+      i. des.
+      esplits; eauto. econs; i.
+      - revert GET_SRC. erewrite Memory.lower_o; eauto. condtac; ss.
+        + i. des. inv GET_SRC.
+          erewrite Memory.lower_o; eauto. condtac; ss.
+          esplits; eauto. refl.
+        + i. erewrite Memory.lower_o; eauto. condtac; ss. eauto.
+      - revert GET_TGT. erewrite Memory.lower_o; eauto. condtac; ss.
+        + i. des. inv GET_TGT.
+          erewrite Memory.lower_o; eauto. condtac; ss.
+          esplits; eauto. refl.
+        + i. erewrite Memory.lower_o; eauto. condtac; ss. eauto.
+      - exploit REL_WRITES; eauto. i. des.
+        erewrite Memory.lower_o; eauto.
+        erewrite (@Memory.lower_o mem2_tgt); eauto.
+        condtac; ss; eauto.
+        des. subst. esplits; eauto.
+    Qed.
+
+    Lemma sim_memory_remove
+          tr mem1_src
+          mem1_tgt loc from to msg mem2_tgt
+          (SIM1: sim_memory tr mem1_src mem1_tgt)
+          (LOC: L loc = false)
+          (REL_WRITE: forall th e
+                        (IN: List.In (th, e) tr)
+                        (REL_WRITE: rel_write e = Some (loc, to)),
+              False)
+          (REMOVE_TGT: Memory.remove mem1_tgt loc from to msg mem2_tgt):
+      exists mem2_src,
+        <<REMOVE_SRC: Memory.remove mem1_src loc from to msg mem2_src>> /\
+        <<SIM2: sim_memory tr mem2_src mem2_tgt>>.
+    Proof.
+      inv SIM1.
+      exploit (@Memory.remove_exists mem1_src loc from to msg).
+      { exploit Memory.remove_get0; eauto. i. des.
+        exploit COMPLETE; eauto. i. des.
+        inv MSG; ss. rewrite LOC in *. subst. ss. }
+      i. des.
+      esplits; eauto. econs; i.
+      - revert GET_SRC. erewrite Memory.remove_o; eauto. condtac; ss.
+        i. erewrite Memory.remove_o; eauto. condtac; ss. eauto.
+      - revert GET_TGT. erewrite Memory.remove_o; eauto. condtac; ss.
+        i. erewrite Memory.remove_o; eauto. condtac; ss. eauto.
+      - exploit REL_WRITES; eauto. i. des.
+        erewrite Memory.remove_o; eauto.
+        erewrite (@Memory.remove_o mem2_tgt); eauto.
+        condtac; ss; eauto.
+        des. subst. exploit REL_WRITE; eauto. ss.
+    Qed.
+
+    Lemma promise_step
+          tr lc1_src mem1_src
+          lc1_tgt mem1_tgt loc from to msg lc2_tgt mem2_tgt kind
+          (LC1: sim_local tr lc1_src lc1_tgt)
+          (MEM1: sim_memory tr mem1_src mem1_tgt)
+          (WF1_SRC: Local.wf lc1_src mem1_src)
+          (WF1_TGT: Local.wf lc1_src mem1_tgt)
+          (STEP_TGT: Local.promise_step lc1_tgt mem1_tgt loc from to msg lc2_tgt mem2_tgt kind)
+          (RESERVE: L loc -> msg = Message.reserve):
+      exists lc2_src mem2_src,
+        <<STEP_SRC: Local.promise_step lc1_src mem1_src loc from to msg lc2_src mem2_src kind>> /\
+        <<LC2: sim_local tr lc2_src lc2_tgt>> /\
+        <<MEM2: sim_memory tr mem2_src mem2_tgt>>.
+    Proof.
+      destruct (L loc) eqn:LOC.
+      { (* promise on L *)
+        rewrite RESERVE in *; ss.
+        inv LC1. inv MEM1. inv STEP_TGT. inv PROMISE.
+        - (* add *)
+          exploit (@Memory.add_exists mem1_src loc from to Message.reserve).
+          { ii. inv LHS. inv RHS. ss.
+            exploit SOUND; eauto. i. des.
+            exploit Memory.add_get0; try exact MEM. i. des.
+            exploit Memory.add_get1; try exact GET_TGT; eauto. i.
+            exploit Memory.get_ts; try exact GET0. i. des.
+            { subst. timetac. }
+            exploit Memory.get_ts; try exact x1. i. des.
+            { subst. timetac. }
+            exploit Memory.get_disjoint; [exact GET0|exact x1|..]. i. des.
+            { subst. congr. }
+            apply (x4 x); econs; ss. }
+          { inv MEM. inv ADD. ss. }
+          { econs. }
+          i. des.
+          exploit Memory.add_exists_le; try eapply WF1_SRC; eauto. i. des.
+          esplits.
+          + econs; [econs; eauto|..]; ss.
+          + econs; ss.
+            * rewrite PROMISES in *.
+              eapply Memory.add_inj; eauto.
+            * ii. revert PROMISE.
+              erewrite Memory.add_o; eauto. condtac; ss. eauto.
+            * i. erewrite Memory.add_o; eauto. condtac; ss; eauto. des. subst.
+              exploit REL_WRITES; eauto. i. des.
+              exploit Memory.add_get0; try exact MEM. i. des. congr.
+          + econs; i.
+            * revert GET_SRC. erewrite Memory.add_o; eauto. condtac; ss.
+              { i. des. inv GET_SRC.
+                exploit Memory.add_get0; try exact MEM. i. des.
+                esplits; eauto. econs. }
+              { i. erewrite Memory.add_o; eauto. condtac; ss; eauto. }
+            * revert GET_TGT. erewrite Memory.add_o; eauto. condtac; ss.
+              { i. des. inv GET_TGT.
+                exploit Memory.add_get0; try exact x0. i. des.
+                esplits; eauto. econs. }
+              { i. erewrite Memory.add_o; eauto. condtac; ss; eauto. }
+            * exploit REL_WRITES; eauto. i. des.
+              erewrite Memory.add_o; eauto.
+              erewrite (@Memory.add_o mem2_tgt); eauto.
+              condtac; ss; eauto. des. subst.
+              exploit Memory.add_get0; try exact MEM. i. des. congr.
+        - (* split *)
+          des. ss.
+        - (* lower *)
+          des. subst. inv MEM. inv LOWER. inv MSG_LE.
+        - (* cancel *)
+          rewrite <- PROMISES in *.
+          exploit Memory.remove_get0; try exact PROMISES0. i. des.
+          exploit Memory.remove_exists_le; try eapply WF1_SRC; eauto. i. des.
+          esplits.
+          + econs; [econs; eauto|..]; ss.
+          + econs; ss.
+            * ii. revert PROMISE.
+              erewrite Memory.remove_o; eauto. condtac; ss; eauto.
+            * i. erewrite Memory.remove_o; eauto. condtac; ss; eauto.
+          + econs; i.
+            * revert GET_SRC. erewrite Memory.remove_o; eauto. condtac; ss. i.
+              erewrite Memory.remove_o; eauto. condtac; ss. eauto.
+            * revert GET_TGT. erewrite Memory.remove_o; eauto. condtac; ss. i.
+              erewrite Memory.remove_o; eauto. condtac; ss. eauto.
+            * exploit REL_WRITES; eauto. i. des.
+              erewrite Memory.remove_o; eauto.
+              erewrite (@Memory.remove_o mem2_tgt); eauto.
+              condtac; ss; eauto. des. subst.
+              exploit REL_WRITES_NONE; eauto. i.
+              exploit Memory.remove_get0; try exact PROMISES0. i. des. congr.
+      }
+
+      (* promises on other loc *)
+      clear RESERVE. inv LC1. inv STEP_TGT.
+      rewrite <- PROMISES in *. inv PROMISE.
+      - (* add *)
+        exploit sim_memory_add; eauto. i. des.
+        inv MEM1. esplits.
+        + econs; [econs; eauto|..]; ss.
+          * i. subst. exploit SOUND; eauto. i. des. eauto.
+          * eapply sim_memory_closed_message; eauto.
+        + admit.
+        + ss.
+      - (* split *)
+        exploit sim_memory_split; eauto. i. des.
+        inv MEM1. esplits.
+        + econs; [econs; eauto|..]; ss.
+          eapply sim_memory_closed_message; eauto.
+        + admit.
+        + ss.
+      - (* lower *)
+        exploit sim_memory_lower; eauto. i. des.
+        inv MEM1. esplits.
+        + econs; [econs; eauto|..]; ss.
+          eapply sim_memory_closed_message; eauto.
+        + admit.
+        + ss.
+      - (* cancel *)
+        exploit sim_memory_remove; eauto.
+        { i. exploit REL_WRITES_NONE; eauto. i.
+          exploit Memory.remove_get0; try exact PROMISES0. i. des. congr. }
+        i. des.
+        inv MEM1. esplits.
+        + econs; [econs; eauto|..]; ss.
+        + admit.
+        + ss.
+    Admitted.
+
+    Lemma sim_thread_step
+          tr e1_src e1_tgt
+          pf e_tgt e2_tgt
+          (SIM1: sim_thread tr e1_src e1_tgt)
+          (WF1_SRC: Local.wf e1_src.(Thread.local) e1_src.(Thread.memory))
+          (WF1_TGT: Local.wf e1_tgt.(Thread.local) e1_tgt.(Thread.memory))
+          (SC1_SRC: Memory.closed_timemap e1_src.(Thread.sc) e1_src.(Thread.memory))
+          (SC1_TGT: Memory.closed_timemap e1_tgt.(Thread.sc) e1_tgt.(Thread.memory))
+          (MEM1_SRC: Memory.closed e1_src.(Thread.memory))
+          (MEM1_TGT: Memory.closed e1_tgt.(Thread.memory))
+          (STEP_TGT: Thread.step pf e_tgt e1_tgt e2_tgt)
+          (PROMISES_TGT: reserve_only e2_tgt.(Thread.local).(Local.promises)):
+      (True) \/
+      (exists e_src e2_src,
+          <<STEP_SRC: Thread.step pf e_src e1_src e2_src>> /\
+          <<SIM2: sim_thread ((e1_src, e_src) :: tr) e2_src e2_tgt>> /\
+          <<EVENT: ThreadEvent.get_machine_event e_src = ThreadEvent.get_machine_event e_tgt>>).
+    Proof.
+    Admitted.
   End RASimThread.
 End RASimThread.
